
$$
\begin{align}
&\text{Suppose $f(x)$ and $g(x)$ are even.} \\ \\
&h(x)=f(x)\pm g(x) &&h(-x)=f(-x)\pm g(-x)=f(x) \pm g(x)=h(x) \\
&h(x)=f(x)g(x) &&h(-x)=f(-x)g(-x)=f(x)g(x)=h(x) \\ \\
&\text{Suppose $f(x)$ is even and $g(x)$ is odd} \\ \\
&h(x)=f(x)+g(x) &&h(-x)=f(-x)+g(-x)=f(x)-g(x) \\
&h(x)={f(x) \over g(x)} &&h(-x)={f(-x) \over g(-x)}={f(x) \over -g(x)}=-{f(x) \over g(x)}=-h(x) \\ \\
&\text{Suppose $f(x)$ and $g(x)$ are odd} \\ \\
&h(x)=f(x)+g(x) &&h(-x)=f(-x)+g(-x)=-f(x)-g(x)=-(f(x)+g(x))=-h(x) \\
&h(x)=f(x)-g(x) &&h(-x)=f(-x)-g(-x)=-f(x)+g(x)=-(f(x)-g(x))=-h(x) \\
&h(x)=f(x)g(x) &&h(-x)=f(-x)g(-x)=f(x)g(x)=h(x) \\
\end{align}
$$
