$log_a(AB)=log_a(A)+log_a(B)$
Let $A=a^u$ and $B=a^v$ $\quad \therefore \quad$ $u=log_a(A) \text{ and } v=log_a(B)$$log_a(AB)=log_a(a^ua^v)=log_a(a^{u+v})=u+v=log_a(A)+log_a(B)$
$log_a(A)=log_a(B \cdot {A \over B})=log_a(B)+log_a({A \over B})$
$log_a({A \over B})=log_a(A)-log_a(B)$

$log_a(A^c)=log_a((a^u)^c)=log_a(a^{uc})=u\cdot c=c \cdot log_a(A)$


##### Change of Base Formula
$$ 
\begin{align}
y&=log_a(x) \implies a^y=x \\
log_b(a^y)&=log_b(x) \\
y \ log_b(a)&=log_b(x) \\
y=log_a(x)&={log_b(x) \over log_b(a)}
\end{align}
$$
Keep in mind that $a$ and $b$ can be any real 